src/tc/rel.fsi
@@ -33,5 +33,5 @@ val keq : env -> option<typ> -> knd -> knd -> guard
 val teq : env -> typ -> typ -> guard
 val try_subtype: env -> typ -> typ -> option<guard>
 val subtype: env -> typ -> typ -> guard
-val trivial_subtype: env -> typ -> typ -> unit
+val trivial_subtype: env -> option<exp> -> typ -> typ -> unit
 val sub_comp_typ: env -> comp_typ -> comp_typ -> option<guard>
